Proof of parralel reduction

LambdaCalculus.v
@@ -1,9 +1,9 @@
 Require Import Arith.
 
-Inductive scoped_term {scope : nat} : Set :=
-| TVar : nat -> @scoped_term scope
-| TApp : @scoped_term scope -> @scoped_term scope -> @scoped_term scope
-| TAbstr : @scoped_term (S scope) -> @scoped_term scope.
+Inductive term : Set :=
+| TVar : nat -> term
+| TApp : term -> term -> term
+| TAbstr : term -> term.
 
 (*
 Inductive appears_free_in (x : identifier) : term -> Prop :=
@@ -30,18 +30,17 @@ Inductive appears_bound_in (x : identifier) : term -> Prop :=
 
 Reserved Notation "'[' x ':=' s ']' t" (at level 20).
 
-Fixpoint rescope {scope : nat} (s : @scoped_term scope) (deep: nat) : @scoped_term (S scope) :=
+Fixpoint rescope (s : term) (deep: nat) : term :=
   match s with
     | TVar k =>
-      if le_lt_dec deep k
+      if leb deep k
       then TVar (S k)
       else TVar k
     | TApp t1 t2 => TApp (rescope t1 deep) (rescope t2 deep)
     | TAbstr t => TAbstr (rescope t (S deep))
   end.
 
-Fixpoint subst {scope : nat}
-         (var : nat) (s : @scoped_term scope) (t : @scoped_term (S scope)) :=
+Fixpoint subst (var : nat) (s : term) (t : term) :=
   match t with
     | TApp t1 t2 => TApp (subst var s t1) (subst var s t2)
     | TVar v =>
@@ -56,19 +55,25 @@ Fixpoint subst {scope : nat}
 where "'[' x ':=' s ']' t" := (subst x s t).
 
 
-Reserved Notation "u '==>' v" (at level 20).
+Reserved Notation "u '-->' v" (at level 20).
 
-Inductive beta_reduction {s : nat} : @scoped_term s -> @scoped_term s -> Prop :=
-| BApp1 : forall (t1 t1' t2 : @scoped_term s),
+Inductive beta_reduction : term -> term -> Prop :=
+| b_app1 : forall (t1 t1' t2 : term),
             beta_reduction t1 t1' ->
             beta_reduction (TApp t1 t2) (TApp t1' t2)
-| BApp2 : forall (t1 t2 t2' : @scoped_term s),
+| b_app2 : forall (t1 t2 t2' : term),
             beta_reduction t2 t2' ->
             beta_reduction (TApp t1 t2) (TApp t1 t2')
-| BRed : forall (u : @scoped_term (S s)) (v : @scoped_term s),
-           beta_reduction (TApp (TAbstr u) v) ([0 := v]u).
+| b_abstr : forall (u u' : term),
+             beta_reduction u u' ->
+             beta_reduction (TAbstr u) (TAbstr u')
+| b_red : forall (u : term) (v : term),
+            beta_reduction (TApp (TAbstr u) v) ([0 := v]u)
 
-Module Confluence.
+where "u '-->' v" := (beta_reduction u v).
+
+
+Section Confluence.
   Require Import Relation_Definitions.
   Require Import Operators_Properties.
   Require Import Relation_Operators.
@@ -282,3 +287,371 @@ Lemma strongly_length :
     apply strongly_length with (n:=n) (x:=x) ; assumption.
   Qed.
 End Confluence.
+
+Require Import Operators_Properties.
+Require Import Relation_Operators.
+
+Definition beta_star :=
+  RStar term beta_reduction.
+
+Notation "u '-->*' v" := (beta_star u v) (at level 20).
+
+
+Lemma b_app1_star :
+  forall (t1 t1' t2: term),
+    t1 -->* t1' ->
+    (TApp t1 t2) -->* (TApp t1' t2).
+Proof.
+  intros t1 t1' t2 H1. induction H1.
+  - apply rt1n_refl.
+  - apply rt1n_trans with (TApp y t2) ; [constructor | idtac] ; assumption.
+Qed.
+
+Lemma b_app2_star :
+  forall (t1 t2 t2': term),
+    t2 -->* t2' ->
+    (TApp t1 t2) -->* (TApp t1 t2').
+Proof.
+  intros t1 t2 t2' H2. induction H2.
+  - apply rt1n_refl.
+  - apply rt1n_trans with (TApp t1 y) ; [constructor | idtac] ; assumption.
+Qed.
+
+Lemma b_abstr_star :
+  forall (t1 t1': term),
+    t1 -->* t1' ->
+    (TAbstr t1) -->* (TAbstr t1').
+Proof.
+  intros t1 t1' H1. induction H1.
+  - apply rt1n_refl.
+  - apply rt1n_trans with (TAbstr y) ; [constructor | idtac] ; assumption.
+Qed.
+
+Module Parallel.
+  Require Import Omega.
+  Hint Resolve nat_compare_eq_iff.
+  Hint Resolve nat_compare_lt.
+  Hint Resolve nat_compare_gt.
+  Hint Resolve nat_compare_Lt_lt.
+  Hint Resolve nat_compare_Gt_gt.
+
+
+  Reserved Notation "u '==>' v" (at level 20).
+
+  Inductive par_reduction : term -> term -> Prop :=
+  | p_app : forall (t1 t1' t2 t2' : term),
+             t1 ==> t1' ->
+             t2 ==> t2' ->
+             (TApp t1 t2) ==> (TApp t1' t2')
+  | p_id : forall (u : term),
+             u ==> u
+  | p_abstr : forall (u u' : term),
+               u ==> u' ->
+               (TAbstr u) ==> (TAbstr u')
+  | p_red : forall (u u' : term) (v v' : term),
+             u ==> u' ->
+             v ==> v' ->
+             (TApp (TAbstr u) v) ==> ([0 := v']u')
+  where "u '==>' v" := (par_reduction u v).
+
+  Hint Constructors par_reduction.
+
+  Lemma beta_implies_par :
+    forall (a b : term),
+      a --> b -> a ==> b.
+  Proof.
+    intros a b H. induction H.
+    - apply p_app. assumption. apply p_id.
+    - apply p_app. apply p_id. assumption.
+    - apply p_abstr. assumption.
+    - apply p_red ; apply p_id.
+  Qed.
+
+  Lemma par_implies_beta_star :
+    forall (a b : term),
+      a ==> b -> a -->* b.
+  Proof.
+    intros a b H. induction H.
+    - apply rstar_trans with (TApp t1' t2) ;
+      [apply b_app1_star | apply b_app2_star] ; assumption.
+    - apply rt1n_refl.
+    - apply b_abstr_star ; assumption.
+    - apply rstar_trans with (TApp (TAbstr u') v').
+      apply rstar_trans with (TApp (TAbstr u') v).
+      apply b_app1_star. apply b_abstr_star. assumption.
+      apply b_app2_star. assumption.
+      apply clos_rt1n_step. apply b_red.
+  Qed.
+
+  Lemma par_refl :
+    forall (u v : term),
+      RRefl term par_reduction u v -> par_reduction u v.
+  Proof.
+    intros u v Hrefl.
+    induction Hrefl.
+    - apply p_id.
+    - assumption.
+  Qed.
+
+  Lemma subs_rescope :
+    forall (k : nat) (u v : term),
+      [k := v](rescope u k) = u.
+  Proof.
+    intros k u. generalize dependent k.
+    induction u ; intros k v.
+
+    - simpl.
+      destruct (leb k n) eqn:Eq.
+      + assert (nat_compare k (S n) = Lt).
+        apply nat_compare_lt. apply le_n_S. apply leb_complete. assumption.
+        simpl. rewrite H. reflexivity.
+      + assert (nat_compare k n = Gt).
+        apply nat_compare_gt. apply leb_complete_conv. assumption.
+        simpl. rewrite H. reflexivity.
+    - simpl. rewrite IHu1. rewrite IHu2. reflexivity.
+    - simpl. rewrite IHu. reflexivity.
+  Qed.
+
+  Lemma rescope_comm :
+    forall (v : term) (j k : nat),
+      k <= j -> rescope (rescope v j) k = rescope (rescope v k) (S j).
+  Proof with auto.
+    intros v.
+    induction v ; intros j k Hjk.
+    - unfold rescope.
+      destruct (leb j n) eqn:E1.
+      + assert (j <= n). apply le_S_n. apply leb_complete. assumption.
+        assert (leb j n = true). apply leb_correct. assumption.
+        assert (leb k n = true). apply leb_correct. omega.
+        assert (leb k (S n) = true). apply leb_correct. omega.
+        assert (leb (S j) (S n) = true). apply leb_correct. omega.
+        simpl. rewrite H1. rewrite H2. rewrite H3. reflexivity.
+      + destruct (leb k n).
+        * assert (j > n). apply leb_complete_conv. assumption.
+          assert (leb (S j) (S n) = false). apply leb_correct_conv. omega.
+          rewrite H0. reflexivity.
+        * assert (j > n). apply leb_complete_conv. assumption.
+          assert (leb (S j) n = false). apply leb_correct_conv. omega.
+          rewrite H0. reflexivity.
+    - simpl. rewrite IHv1... rewrite IHv2...
+    - simpl. rewrite IHv... omega.
+  Qed.
+
+  Lemma rescope_factorization :
+    forall (k : nat) (u v : term) (d : nat),
+      d <= k ->
+      ([S k := rescope v d]rescope u d) = rescope ([k := v]u) d.
+  Proof with auto.
+    intros k u. generalize dependent k.
+    induction u ; intros k v d Hdk.
+    - simpl.
+      destruct (nat_compare k n) eqn:E.
+      + assert (k = n). apply nat_compare_eq_iff. assumption. subst.
+        replace (leb d n) with true. simpl. rewrite E. reflexivity.
+        symmetry. apply leb_correct. assumption.
+      + simpl.
+        assert (k < n). apply nat_compare_lt. assumption.
+        replace (leb d (pred n)) with true.
+        replace (leb d n) with true.
+        simpl. rewrite E.
+        rewrite <- S_pred with n k. reflexivity.
+        assumption.
+        symmetry. apply leb_correct. omega.
+        symmetry. apply leb_correct. omega.
+      + simpl. destruct (leb d n) ; unfold subst.
+        * rewrite nat_compare_S. rewrite E. reflexivity.
+        * assert (nat_compare (S k) n = Gt).
+          apply nat_compare_gt. apply le_S. apply nat_compare_Gt_gt. assumption.
+          rewrite H. reflexivity.
+    - simpl. rewrite IHu1... rewrite IHu2...
+    - simpl. rewrite rescope_comm. rewrite IHu. reflexivity.
+      omega. omega.
+  Qed.
+
+  Lemma rescope_factorization' :
+    forall (k : nat) (u v : term) (d : nat),
+      k <= d ->
+      ([k := rescope v d]rescope u (S d)) = rescope ([k := v]u) d.
+  Proof with auto.
+    intros k u. generalize dependent k.
+    induction u ; intros k v d Hkd.
+    - destruct (nat_compare k n) eqn:E.
+      + assert (k = n). apply nat_compare_eq. assumption. subst.
+        assert (leb (S d) n = false). apply leb_correct_conv. omega.
+        unfold rescope. rewrite H. simpl. rewrite E. reflexivity.
+      + assert (k < n). apply nat_compare_lt. assumption.
+        unfold rescope.
+        destruct (leb (S d) n) eqn:Eq.
+        * simpl. rewrite E.
+          assert (nat_compare k (S n) = Lt). apply nat_compare_lt. omega.
+          assert (S d <= n). apply leb_complete. assumption.
+          assert (leb d (pred n) = true). apply leb_correct. omega.
+          rewrite H0. rewrite H2. replace (S (pred n)) with n. reflexivity.
+          omega.
+        * fold rescope. unfold subst. rewrite E.
+          unfold rescope.
+          assert (n < (S d)). apply leb_complete_conv. assumption.
+          assert (leb d (pred n) = false). apply leb_correct_conv. omega.
+          rewrite H1. reflexivity.
+      + assert (k > n). apply nat_compare_gt. assumption.
+        unfold rescope, subst. rewrite E.
+        assert (leb d n = false). apply leb_correct_conv. omega.
+        assert (leb (S d) n = false). apply leb_correct_conv. omega.
+        rewrite H0. rewrite H1. rewrite E. reflexivity.
+    - simpl. rewrite IHu1... rewrite IHu2...
+    - simpl. rewrite rescope_comm. rewrite IHu...
+      omega. omega.
+  Qed.
+
+  Lemma subst_commutator :
+    forall (k j: nat) (v1 v2 : term) (u : term),
+      j <= k -> [k := v1]([j := v2]u) = [j := [k := v1]v2]([S k := rescope v1 j]u).
+  Proof with auto.
+    intros k j v1 v2 u.
+    generalize dependent v2. generalize dependent v1. generalize dependent j.
+    generalize dependent k.
+    induction u ; intros k j v1 v2 Hjk.
+    - unfold subst. destruct (nat_compare (S k) n) eqn:E1.
+      + fold subst. rewrite subs_rescope.
+        assert (S k = n). apply nat_compare_eq_iff. assumption.
+        subst.
+        assert (nat_compare j (S k) = Lt). apply nat_compare_lt. omega.
+        rewrite H. simpl. rewrite <- nat_compare_S. rewrite E1. reflexivity.
+      + fold subst.
+        assert ((S k) < n). apply nat_compare_lt. assumption.
+        assert (nat_compare j (pred n) = Lt). apply nat_compare_lt. omega.
+        assert (nat_compare j n = Lt). apply nat_compare_lt. omega.
+        rewrite H0. rewrite H1. simpl.
+        assert (nat_compare k (pred n) = Lt). apply nat_compare_lt. omega.
+        rewrite H2. reflexivity.
+      + fold subst. assert (S k > n). apply nat_compare_gt. assumption.
+        destruct (nat_compare j n) eqn:E2...
+        * assert (j < n). apply nat_compare_lt. assumption.
+          simpl.
+          assert (nat_compare k (pred n) = Gt). apply nat_compare_gt. omega.
+          rewrite H1. reflexivity.
+        * assert (n < j). apply nat_compare_gt. assumption. simpl.
+          assert (nat_compare k n = Gt). apply nat_compare_gt. omega.
+          rewrite H1. reflexivity.
+    - simpl. rewrite IHu1... rewrite IHu2...
+    - simpl. rewrite IHu... rewrite rescope_factorization...
+      pattern (rescope (rescope v1 j) 0). rewrite rescope_comm.
+      reflexivity. omega. omega. omega.
+  Qed.
+
+
+  Lemma rescope_par :
+    forall (v v' : term) (k : nat),
+      v ==> v' -> rescope v k ==> rescope v' k.
+  Proof with auto.
+    intros v v' k Hv. generalize dependent k.
+    induction Hv ; intros k ; simpl...
+    - rewrite <- rescope_factorization'. apply p_red... omega.
+  Qed.
+
+  Lemma subs_par_id :
+    forall u (v v' : term) (k : nat),
+    par_reduction v v' ->
+    par_reduction ([k := v]u) ([k := v']u).
+  Proof with auto.
+    intros u. induction u ; intros v v' k Hv.
+    - unfold subst.
+      destruct (nat_compare k n) ; subst ; try (apply p_id)...
+    - simpl. apply p_app...
+    - simpl. apply p_abstr... apply IHu. apply rescope_par...
+  Qed.
+
+  Lemma par_abstr_inv :
+    forall (u v : term),
+      TAbstr u ==> v -> exists u', u ==> u' /\ v = TAbstr u'.
+  Proof.
+    intros u v H.
+    inversion H ; subst.
+    - exists u. split ; auto.
+    - exists u'. split ; auto.
+  Qed.
+
+  Lemma subst_par :
+    forall (u u' : term) (v v' : term) (k : nat),
+      par_reduction u u' ->
+      par_reduction v v' ->
+      par_reduction ([k := v]u) ([k := v']u').
+  Proof with auto.
+    intros u u' v v' k Hu.
+    generalize dependent k. generalize dependent v'. generalize dependent v.
+    induction Hu ; intros w w' k Hv.
+    - simpl. apply p_app...
+    - simpl. apply subs_par_id...
+    - simpl. apply p_abstr... apply IHHu. apply rescope_par...
+    - simpl. rewrite subst_commutator. apply p_red...
+      apply IHHu1. apply rescope_par... omega.
+  Qed.
+
+  Lemma par_strongly_confluent :
+    strongly_confluent term par_reduction.
+  Proof with auto.
+    intros x y z Hxy. generalize dependent z.
+    induction Hxy ; intros z Hxz.
+    - inversion Hxz ; subst.
+      + elim (IHHxy1 t1'0 H1).
+        elim (IHHxy2 t2'0 H3).
+        intros w2 [H2' H2'0] w1 [H1' H1'0].
+        exists (TApp w1 w2).
+        split ; apply r_step ; (apply p_app ; apply par_refl ; assumption).
+      + exists (TApp t1' t2').
+        split ; apply r_step ; [apply p_id | apply p_app ; assumption].
+      + elim (IHHxy1 (TAbstr u')).
+        elim (IHHxy2 v' H3).
+        intros w2 [H2' H2'0] w1 [H1' H1'0].
+        apply par_refl in H1'0.
+        elim (par_abstr_inv u' w1 H1'0).
+        intros w1' [Huw1' Hw1w1']. subst.
+        exists ([0 := w2]w1').
+        elim (par_abstr_inv u t1' Hxy1).
+        intros s [Hus Ht1's]. subst.
+        apply par_refl in H2'.
+        apply par_refl in H2'0.
+        apply par_refl in H1'. inversion H1'. subst.
+        * split ; apply r_step.
+          apply p_red...
+          apply subst_par...
+        * split ; apply r_step.
+          apply p_red...
+          apply subst_par...
+        * constructor...
+   - exists z. split ; apply r_step...
+   - elim (par_abstr_inv u z Hxz).
+     intros v [Huv Hv]. subst.
+     elim (IHHxy v Huv).
+     intros w [Hu'x Hvx].
+     exists (TAbstr w).
+     apply par_refl in Hu'x.
+     apply par_refl in Hvx.
+     split ; apply r_step...
+   - inversion Hxz ; subst.
+     + elim (par_abstr_inv u t1' H1).
+       intros x [Hux Ht1'x]. subst.
+       elim (IHHxy2 t2' H3).
+       elim (IHHxy1 x Hux).
+       intros u0 [Hu'u0 Hxu0] v0 [Hv'v0 Ht2'v0].
+       apply par_refl in Hu'u0.
+       apply par_refl in Hxu0.
+       apply par_refl in Hv'v0.
+       apply par_refl in Ht2'v0.
+       exists ([0 := v0]u0).
+       split ; apply r_step...
+       apply subst_par...
+     + exists ([0 := v']u').
+       split ; apply r_step...
+     + elim (IHHxy2 v'0 H3).
+       elim (IHHxy1 u'0 H1).
+       intros u0 [Hu'u0 Hu'0u0] v0 [Hv'v0 Hv'0v0].
+       apply par_refl in Hu'u0.
+       apply par_refl in Hu'0u0.
+       apply par_refl in Hv'v0.
+       apply par_refl in Hv'0v0.
+       exists ([0 := v0]u0).
+       split ; apply r_step ; apply subst_par...
+  Qed.
+
+End Parallel.
